New compiler.

driver/CompilerExtra.v
@@ -71,133 +71,413 @@ Require Linearizeproof.
 Require CleanupLabelsproof.
 Require Stackingproof.
 Require Asmgenproof.
+
 Require Import Compiler.
-Require Import sflib.
+(** Command-line flags. *)
+Require Import Compopts.
 
-Definition transf_cminor_program_to_rtl (p: Cminor.program) : res RTL.program :=
-   OK p
-   @@ print print_Cminor
-  @@@ time "Instruction selection" Selection.sel_program
-  @@@ time "RTL generation" RTLgen.transl_program.
+(** Pretty-printers (defined in Caml). *)
+(* Parameter print_Clight: Clight.program -> unit. *)
+(* Parameter print_Cminor: Cminor.program -> unit. *)
+(* Parameter print_RTL: Z -> RTL.program -> unit. *)
+(* Parameter print_LTL: LTL.program -> unit. *)
+(* Parameter print_Mach: Mach.program -> unit. *)
 
-Definition transf_clight_program_to_rtl (p: Clight.program) : res RTL.program :=
-  OK p 
-   @@ print print_Clight
-  @@@ time "Simplification of locals" SimplLocals.transf_program
-  @@@ time "C#minor generation" Cshmgen.transl_program
-  @@@ time "Cminor generation" Cminorgen.transl_program
-  @@@ transf_cminor_program_to_rtl.
+Open Local Scope string_scope.
 
-Definition transf_c_program_to_rtl (p: Csyntax.program) : res RTL.program :=
-  OK p 
-  @@@ time "Clight generation" SimplExpr.transl_program
-  @@@ transf_clight_program_to_rtl.
+(** * Composing the translation passes *)
 
-Definition transf_rtl_program_to_asm (f: RTL.program) : res Asm.program :=
-   OK f
-   @@ print (print_RTL 0)
-   @@@ time "Register allocation" Allocation.transf_program
+(** We first define useful monadic composition operators,
+    along with funny (but convenient) notations. *)
+
+(* Definition apply_total (A B: Type) (x: res A) (f: A -> B) : res B := *)
+(*   match x with Error msg => Error msg | OK x1 => OK (f x1) end. *)
+
+(* Definition apply_partial (A B: Type) *)
+(*                          (x: res A) (f: A -> res B) : res B := *)
+(*   match x with Error msg => Error msg | OK x1 => f x1 end. *)
+
+(* Notation "a @@@ b" := *)
+(*    (apply_partial _ _ a b) (at level 50, left associativity). *)
+(* Notation "a @@ b" := *)
+(*    (apply_total _ _ a b) (at level 50, left associativity). *)
+
+(* Definition print {A: Type} (printer: A -> unit) (prog: A) : A := *)
+(*   let unused := printer prog in prog. *)
+
+(* Definition time {A B: Type} (name: string) (f: A -> B) : A -> B := f. *)
+
+(* Definition total_if {A: Type} *)
+(*           (flag: unit -> bool) (f: A -> A) (prog: A) : A := *)
+(*   if flag tt then f prog else prog. *)
+
+(* Definition partial_if {A: Type} *)
+(*           (flag: unit -> bool) (f: A -> res A) (prog: A) : res A := *)
+(*   if flag tt then f prog else OK prog. *)
+
+Inductive rtl_pass: Type :=
+| Tailcall: rtl_pass
+| Inlining: rtl_pass
+| Renumber: rtl_pass
+| Constprop: rtl_pass
+| CSE: rtl_pass
+| Deadcode: rtl_pass.
+
+Definition opt_list:= list (rtl_pass * (unit -> bool)).
+Definition tflag := (fun (t:unit) => true).
+Definition fflag := (fun (t:unit) => false).
+
+
+(** We define three translation functions for whole programs: one
+  starting with a C program, one with a Cminor program, one with an
+  RTL program.  The three translations produce Asm programs ready for
+  pretty-printing and assembling. *)
+
+Definition transf_rtl_program_to_asm_opt (p: res RTL.program) : res Asm.program :=
+   p
+   @@ print (print_RTL 7)
+  @@@ time "Register allocation" Allocation.transf_program
    @@ print print_LTL
    @@ time "Branch tunneling" Tunneling.tunnel_program
-  @@@ Linearize.transf_program
+  @@@ time "CFG linearization" Linearize.transf_program
    @@ time "Label cleanup" CleanupLabels.transf_program
   @@@ time "Mach generation" Stacking.transf_program
    @@ print print_Mach
   @@@ time "Asm generation" Asmgen.transf_program.
 
-Inductive optimize_rtl_program: forall (rtl: RTL.program) (ortl: RTL.program), Prop:=
-| rtlopt_tailcall: forall r1,
-                     optimize_rtl_program r1 (Tailcall.transf_program r1)
-| rtlopt_inlining: forall r1 r1' (TR_OK: Inlining.transf_program r1 = OK r1'),
-                     optimize_rtl_program r1 r1'
-| rtlopt_renumber: forall r1,
-                     optimize_rtl_program r1 (Renumber.transf_program r1)
-| rtlopt_constprop: forall r1,
-                      optimize_rtl_program r1 (Constprop.transf_program r1)
-| rtlopt_cse: forall r1 r1' (TR_OK: CSE.transf_program r1 = OK r1'),
-                optimize_rtl_program r1 r1'
-| rtlopt_deadcode: forall r1 r1' (TR_OK: Deadcode.transf_program r1 = OK r1'),
-                     optimize_rtl_program r1 r1'.
 
-Definition compile_c_program (c: Csyntax.program) (a:Asm.program) : Prop :=
-  exists rtl ortl,
-    transf_c_program_to_rtl c = OK rtl
-    /\ (rtc optimize_rtl_program) rtl ortl
-    /\ transf_rtl_program_to_asm ortl = OK a.
-
-Ltac simplify:=
-  match goal with
-    | H: match ?x with
-           | OK _ => _
-           | Error _ => Error _
-         end = OK _
-      |- _ => (destruct x eqn:?D;[|inv H])
-    | H: OK _ = OK _ |- _ => inv H
+Fixpoint transf_rtl_program_opt' (z:Z) (l:opt_list) (p: res RTL.program) : res Asm.program :=
+  match l with
+    | nil =>
+      transf_rtl_program_to_asm_opt p
+    | (pass, flag)::l' =>
+      let p' := p @@ print (print_RTL z) in
+      let p'' :=
+          match pass with
+            | Tailcall => p' @@ total_if flag (time "Tail calls" Tailcall.transf_program)
+            | Inlining => p' @@@ partial_if flag (time "Inlining" Inlining.transf_program)
+            | Renumber => p' @@ total_if flag (time "Renumbering" Renumber.transf_program)
+            | Constprop => p' @@ total_if flag (time "Constant propagation" Constprop.transf_program)
+            | CSE => p' @@@ partial_if flag (time "CSE" CSE.transf_program)
+            | Deadcode => p' @@@ partial_if flag (time "Redundancy elimination" Deadcode.transf_program)
+          end
+      in transf_rtl_program_opt' (z+1) l' p''
   end.
 
-Lemma transf_c_program_compile_c_program:
-  forall p tp
-         (Htrans: transf_c_program p = OK tp),
-    compile_c_program p tp.
+Definition transf_rtl_program_opt (z:Z) (l:opt_list) (p: RTL.program) : res Asm.program :=
+  transf_rtl_program_opt' z l (OK p).
+  
+Definition transf_cminor_program_opt (l:opt_list) (p: Cminor.program) : res Asm.program :=
+  OK p
+  @@ print print_Cminor
+  @@@ time "Instruction selection" Selection.sel_program
+  @@@ time "RTL generation" RTLgen.transl_program
+  @@@ transf_rtl_program_opt 0 l.
+
+Definition transf_clight_program_opt (l: opt_list) (p: Clight.program) : res Asm.program :=
+  OK p
+  @@ print print_Clight
+  @@@ time "Simplification of locals" SimplLocals.transf_program
+  @@@ time "C#minor generation" Cshmgen.transl_program
+  @@@ time "Cminor generation" Cminorgen.transl_program
+  @@@ transf_cminor_program_opt l.
+
+Definition transf_c_program_opt l p : res Asm.program :=
+  OK p
+     @@@ time "Clight generation" SimplExpr.transl_program
+     @@@ transf_clight_program_opt l.
+
+(* Ltac match_solve := *)
+(*   match goal with *)
+(*       [|- match ?x with | OK _ => _ | Error _ => _ end = *)
+(*           match ?x with | OK _ => _ | Error _ => _ end *)
+(*       ] => destruct x; [| reflexivity] *)
+(*   end. *)
+
+(* Lemma OK_apply_partial: *)
+(*   forall A B (f:A -> res B) (a:A), *)
+(*     OK a @@@ f = f a. *)
+(* Proof. eauto. Qed. *)
+
+(* Lemma OK_apply_total: *)
+(*   forall A B (f:A -> B) (a:A), *)
+(*     OK a @@ f = OK (f a). *)
+(* Proof. eauto. Qed. *)
+
+(* Lemma partial_if_tflag: *)
+(*   forall A (f:A -> res A) (a:A), *)
+(*     partial_if tflag f a = f a. *)
+(* Proof. auto. Qed. *)
+
+(* Lemma total_if_tflag: *)
+(*   forall A (f:A -> A) (a:A), *)
+(*     total_if tflag f a = f a. *)
+(* Proof. auto. Qed. *)
+
+Definition compiler_flag :=
+    (Tailcall, optim_tailcalls)::(Inlining, tflag)::(Renumber, tflag)::(Constprop, optim_constprop)
+  ::(Renumber, optim_constprop)::(CSE, optim_CSE)::(Deadcode, optim_redundancy)::nil.
+
+Require Import FunctionalExtensionality.
+
+Theorem compiler_equivalence:
+  transf_c_program = transf_c_program_opt compiler_flag.
+Proof. reflexivity. Qed.
+
+
+
+  (* Lemma same_res_apply_partial: *)
+  (*   forall A B (f1 f2: A -> res B), *)
+  (*     (forall a, f1 a = f2 a) -> *)
+  (*     forall ra, ra @@@ f1 = ra @@@ f2. *)
+  (* Proof. *)
+  (*   intros. *)
+  (*   unfold apply_total. *)
+  (*   destruct ra; try rewrite H; eauto. *)
+  (* Qed. *)
+
+  (* apply same_res_apply_total. *)
+  
+    
+    
+  (*     res1 @@  *)
+  
+  (* unfold apply_total. match_solve. *)
+
+  
+  (* simpl. *)
+
+  (* destruct (optim_tailcalls tt) eqn:Htailcall. *)
+  (* - instantiate (1:= (Tailcall, tflag) :: nil). *)
+  (*   admit. *)
+  (* - instantiate (1:= (Tailcall, fflag) :: nil). *)
+  (*   admit. *)
+  (*   unfold transf_rtl_program_opt. *)
+  (*   |  *)
+  (* instantiate (1:= cons _ _).  *)
+  
+
+(** The following lemmas help reason over compositions of passes. *)
+
+(* Lemma print_identity: *)
+(*   forall (A: Type) (printer: A -> unit) (prog: A), *)
+(*   print printer prog = prog. *)
+(* Proof. *)
+(*   intros; unfold print. destruct (printer prog); auto.  *)
+(* Qed. *)
+
+(* Lemma compose_print_identity: *)
+(*   forall (A: Type) (x: res A) (f: A -> unit),  *)
+(*   x @@ print f = x. *)
+(* Proof. *)
+(*   intros. destruct x; simpl. rewrite print_identity. auto. auto.  *)
+(* Qed. *)
+
+(* Remark forward_simulation_identity: *)
+(*   forall sem, forward_simulation sem sem. *)
+(* Proof. *)
+(*   intros. apply forward_simulation_step with (fun s1 s2 => s2 = s1); intros. *)
+(* - auto. *)
+(* - exists s1; auto. *)
+(* - subst s2; auto. *)
+(* - subst s2. exists s1'; auto.  *)
+(* Qed.  *)
+
+(* Lemma total_if_simulation: *)
+(*   forall (A: Type) (sem: A -> semantics) (flag: unit -> bool) (f: A -> A) (prog: A), *)
+(*   (forall p, forward_simulation (sem p) (sem (f p))) -> *)
+(*   forward_simulation (sem prog) (sem (total_if flag f prog)). *)
+(* Proof. *)
+(*   intros. unfold total_if. destruct (flag tt). auto. apply forward_simulation_identity. *)
+(* Qed. *)
+
+(* Lemma partial_if_simulation: *)
+(*   forall (A: Type) (sem: A -> semantics) (flag: unit -> bool) (f: A -> res A) (prog tprog: A), *)
+(*   partial_if flag f prog = OK tprog -> *)
+(*   (forall p tp, f p = OK tp -> forward_simulation (sem p) (sem tp)) -> *)
+(*   forward_simulation (sem prog) (sem tprog). *)
+(* Proof. *)
+(*   intros. unfold partial_if in *. destruct (flag tt). eauto. inv H. apply forward_simulation_identity. *)
+(* Qed. *)
+
+(** * Semantic preservation *)
+
+(** We prove that the [transf_program] translations preserve semantics
+  by constructing the following simulations:
+- Forward simulations from [Cstrategy] / [Cminor] / [RTL] to [Asm]
+  (composition of the forward simulations for each pass).
+- Backward simulations for the same languages
+  (derived from the forward simulation, using receptiveness of the source
+  language and determinacy of [Asm]).
+- Backward simulation from [Csem] to [Asm]
+  (composition of two backward simulations).
+
+These results establish the correctness of the whole compiler! *)
+
+Lemma transf_rtl_program_opt'_error: forall l n msg, transf_rtl_program_opt' n l (Error msg) = Error msg.
+Proof.
+  intros l. induction l; intros; eauto.
+  simpl. destruct a. destruct r; eauto.
+Qed.
+
+Theorem transf_rtl_program_opt_correct:
+  forall n l p tp,
+  transf_rtl_program_opt n l p = OK tp ->
+  forward_simulation (RTL.semantics p) (Asm.semantics tp)
+  * backward_simulation (RTL.semantics p) (Asm.semantics tp).
 Proof.
   intros.
-  unfold transf_c_program in Htrans.
-  unfold transf_clight_program in Htrans.
-  unfold transf_cminor_program in Htrans.
-  unfold Compiler.time, Compiler.print in Htrans.
-  unfold Compiler.apply_partial, Compiler.apply_total in Htrans.
+  assert (F: forward_simulation (RTL.semantics p) (Asm.semantics tp)).
+  { generalize dependent p. generalize dependent n. generalize dependent tp.
+    induction l; intros.
+    - unfold transf_rtl_program_opt in H.
+      simpl in H.
+      unfold transf_rtl_program_to_asm_opt, time in H.
+      repeat rewrite compose_print_identity in H.
+      simpl in H.
+      destruct (Allocation.transf_program p) as [p4|] eqn:?; simpl in H; try discriminate.
+      set (p5 := Tunneling.tunnel_program p4) in *.
+      destruct (Linearize.transf_program p5) as [p6|] eqn:?; simpl in H; try discriminate.
+      set (p7 := CleanupLabels.transf_program p6) in *.
+      destruct (Stacking.transf_program p7) as [p8|] eqn:?; simpl in H; try discriminate.
 
-  unfold compile_c_program.
-  unfold transf_c_program_to_rtl.
-  unfold transf_clight_program_to_rtl.
-  unfold transf_cminor_program_to_rtl.
-  unfold time, print, apply_partial, apply_total.
+      apply compose_forward_simulation with (LTL.semantics p4).
+      apply Allocproof.transf_program_correct; auto.
+      apply compose_forward_simulation with (LTL.semantics p5).
+      apply Tunnelingproof.transf_program_correct.
+      apply compose_forward_simulation with (Linear.semantics p6).
+      apply Linearizeproof.transf_program_correct; auto.
+      apply compose_forward_simulation with (Linear.semantics p7).
+      apply CleanupLabelsproof.transf_program_correct. 
+      apply compose_forward_simulation with (Mach.semantics Asmgenproof0.return_address_offset p8).
+      apply Stackingproof.transf_program_correct.
+      exact Asmgenproof.return_address_exists.
+      auto.
+      apply Asmgenproof.transf_program_correct; eauto.
+    - unfold transf_rtl_program_opt in H.
+      simpl in H.
+      destruct a as [pass flag].
+      destruct pass; unfold print, time in H.
+      + set (p1 := total_if flag Tailcall.transf_program p).
+        apply compose_forward_simulation with (RTL.semantics p1); eauto.
+        apply total_if_simulation. intros. apply Tailcallproof.transf_program_correct.
+        apply Tailcallproof.Tailcall_sepcomp_rel. auto.
+      + set (p1' := partial_if flag Inlining.transf_program p).
+        destruct p1' as [p1|] eqn:Hp1; [| subst; rewrite Hp1 in H; rewrite transf_rtl_program_opt'_error in H; inv H].
+        apply compose_forward_simulation with (RTL.semantics p1);
+          [|eapply IHl; unfold transf_rtl_program_opt; subst; rewrite <- Hp1; eauto].
+        subst.
+        eapply partial_if_simulation; eauto. intros.
+        apply Inliningproof.transf_program_correct; auto. apply Inliningproof.Inlining_sepcomp_rel. auto.
+      + set (p1 := total_if flag Renumber.transf_program p).
+        apply compose_forward_simulation with (RTL.semantics p1); eauto.
+        apply total_if_simulation. intros. apply Renumberproof.transf_program_correct.
+        apply Renumberproof.Renumber_sepcomp_rel. auto.
+      + set (p1 := total_if flag Constprop.transf_program p).
+        apply compose_forward_simulation with (RTL.semantics p1); eauto.
+        apply total_if_simulation. intros. apply Constpropproof.transf_program_correct.
+        apply Constpropproof.Constprop_sepcomp_rel. auto.
+      + set (p1' := partial_if flag CSE.transf_program p).
+        destruct p1' as [p1|] eqn:Hp1; [| subst; rewrite Hp1 in H; rewrite transf_rtl_program_opt'_error in H; inv H].
+        apply compose_forward_simulation with (RTL.semantics p1);
+          [|eapply IHl; unfold transf_rtl_program_opt; subst; rewrite <- Hp1; eauto].
+        subst.
+        eapply partial_if_simulation; eauto. intros.
+        apply CSEproof.transf_program_correct; auto. apply CSEproof.CSE_sepcomp_rel. auto.
+      + set (p1' := partial_if flag Deadcode.transf_program p).
+        destruct p1' as [p1|] eqn:Hp1; [| subst; rewrite Hp1 in H; rewrite transf_rtl_program_opt'_error in H; inv H].
+        apply compose_forward_simulation with (RTL.semantics p1);
+          [|eapply IHl; unfold transf_rtl_program_opt; subst; rewrite <- Hp1; eauto].
+        subst.
+        eapply partial_if_simulation; eauto. intros.
+        apply Deadcodeproof.transf_program_correct; auto. apply Deadcodeproof.Deadcode_sepcomp_rel. auto.
+  }
+  split. auto. 
+  apply forward_to_backward_simulation. auto. 
+  apply RTL.semantics_receptive.
+  apply Asm.semantics_determinate.
+Qed.
 
-  destruct (SimplExpr.transl_program p); [|inversion Htrans].
-  destruct (SimplLocals.transf_program p0); [|inversion Htrans].
-  destruct (Cshmgen.transl_program p1); [|inversion Htrans].
-  destruct (Cminorgen.transl_program p2); [|inversion Htrans].
-  destruct (Selection.sel_program p3); [|inversion Htrans].
-  destruct (RTLgen.transl_program p4); [|inversion Htrans].
-  exists p5. clear -Htrans.
+Theorem transf_cminor_program_opt_correct:
+  forall l p tp,
+  transf_cminor_program_opt l p = OK tp ->
+  forward_simulation (Cminor.semantics p) (Asm.semantics tp)
+  * backward_simulation (Cminor.semantics p) (Asm.semantics tp).
+Proof.
+  intros.
+  assert (F: forward_simulation (Cminor.semantics p) (Asm.semantics tp)).
+  unfold transf_cminor_program_opt, time in H.
+  repeat rewrite compose_print_identity in H.
+  simpl in H. 
+  destruct (Selection.sel_program p) as [p1|] eqn:?; simpl in H; try discriminate.
+  destruct (RTLgen.transl_program p1) as [p2|] eqn:?; simpl in H; try discriminate.
+  eapply compose_forward_simulation. apply Selectionproof.transf_program_correct. monadInv Heqr. destruct x; apply EQ. apply Selectionproof.Selection_sepcomp_rel. eauto.
+  eapply compose_forward_simulation. apply RTLgenproof.transf_program_correct. eassumption.
+  exact (fst (transf_rtl_program_opt_correct _ _ _ _ H)).
 
-  unfold transf_rtl_program in Htrans.
-  unfold Compiler.time, Compiler.apply_partial, Compiler.apply_total, Compiler.print in Htrans.
-  repeat simplify.
+  split. auto. 
+  apply forward_to_backward_simulation. auto. 
+  apply Cminor.semantics_receptive.
+  apply Asm.semantics_determinate.
+Qed.
 
-  unfold Compiler.total_if, Compiler.partial_if in *.
-  eexists. split; auto.
-  split.
-  - assert (Hr1: rtc optimize_rtl_program p5 p17).
-    { destruct (Compopts.optim_tailcalls tt).
-      - econs 3; econs 1; [econs 1 | econs 2; eauto].
-      - econs 1. econs 2. eauto.
-    }
-    assert (Hr2: rtc optimize_rtl_program p17 p9).
-    { destruct (Compopts.optim_CSE tt).
-      - destruct (Compopts.optim_constprop tt).
-        + econs 3. econs 1. econs 3.
-          econs 3. econs 1. econs 4.
-          econs 3. econs 1. econs 3.
-          econs 1. econs 5. eauto.
-        + econs 3. econs 1. econs 3.
-          econs 1. econs 5. eauto.
-      - destruct (Compopts.optim_constprop tt).
-        + econs 3. econs 1. econs 3.
-          econs 3. econs 1. econs 4.
-          econs 1. inv D9. econs 3.
-        + econs 1. inv D9. econs 3.
-    }
-    assert (Hr3: rtc optimize_rtl_program p9 p7).
-    { destruct (Compopts.optim_redundancy tt).
-      - econs 1. econs 6. eauto.
-      - inv D7. econs 2.
-    }
-    econs 3; econs 3; eauto.
-  - clear -D0 D2 D5 Htrans.
-    unfold transf_rtl_program_to_asm.
-    unfold apply_partial, apply_total.
-    unfold time, print.
-    destruct (Allocation.transf_program p7); [|inv D5]. simplify.
-    rewrite D2, D0. auto.
+Theorem transf_clight_program_opt_correct:
+  forall l p tp,
+  transf_clight_program_opt l p = OK tp ->
+  forward_simulation (Clight.semantics1 p) (Asm.semantics tp)
+  * backward_simulation (Clight.semantics1 p) (Asm.semantics tp).
+Proof.
+  intros. 
+  assert (F: forward_simulation (Clight.semantics1 p) (Asm.semantics tp)).
+  revert H; unfold transf_clight_program_opt, time; simpl.
+  rewrite print_identity.
+  caseEq (SimplLocals.transf_program p); simpl; try congruence; intros p0 EQ0.
+  caseEq (Cshmgen.transl_program p0); simpl; try congruence; intros p1 EQ1.
+  caseEq (Cminorgen.transl_program p1); simpl; try congruence; intros p2 EQ2.
+  intros EQ3.
+  eapply compose_forward_simulation. apply SimplLocalsproof.transf_program_correct. eauto.
+  eapply compose_forward_simulation. apply Cshmgenproof.transl_program_correct. eauto.
+  eapply compose_forward_simulation. apply Cminorgenproof.transl_program_correct. eauto.
+  exact (fst (transf_cminor_program_opt_correct _ _ _ EQ3)). 
+
+  split. auto. 
+  apply forward_to_backward_simulation. auto. 
+  apply Clight.semantics_receptive.
+  apply Asm.semantics_determinate.
+Qed.
+
+Theorem transf_cstrategy_program_opt_correct:
+  forall l p tp,
+  transf_c_program_opt l p = OK tp ->
+  forward_simulation (Cstrategy.semantics p) (Asm.semantics tp)
+  * backward_simulation (atomic (Cstrategy.semantics p)) (Asm.semantics tp).
+Proof.
+  intros.
+  assert (F: forward_simulation (Cstrategy.semantics p) (Asm.semantics tp)).
+  revert H; unfold transf_c_program_opt, time; simpl.
+  caseEq (SimplExpr.transl_program p); simpl; try congruence; intros p0 EQ0.
+  intros EQ1.
+  eapply compose_forward_simulation. apply SimplExprproof.transl_program_correct. apply SimplExprproof.SimplExpr_sepcomp_rel. eauto.
+  exact (fst (transf_clight_program_opt_correct _ _ _ EQ1)). 
+
+  split. auto. 
+  apply forward_to_backward_simulation.
+  apply factor_forward_simulation. auto. eapply sd_traces. eapply Asm.semantics_determinate.
+  apply atomic_receptive. apply Cstrategy.semantics_strongly_receptive.
+  apply Asm.semantics_determinate.
+Qed.
+
+Theorem transf_c_program_opt_correct:
+  forall l p tp,
+  transf_c_program_opt l p = OK tp ->
+  backward_simulation (Csem.semantics p) (Asm.semantics tp).
+Proof.
+  intros. 
+  apply compose_backward_simulation with (atomic (Cstrategy.semantics p)).
+  eapply sd_traces; eapply Asm.semantics_determinate.
+  apply factor_backward_simulation. 
+  apply Cstrategy.strategy_simulation.
+  apply Csem.semantics_single_events.
+  eapply ssr_well_behaved; eapply Cstrategy.semantics_strongly_receptive.
+  exact (snd (transf_cstrategy_program_opt_correct _ _ _ H)).
 Qed.
