driver/Linkerproof.v
@@ -63,6 +63,28 @@ Ltac clarify :=
                   apply Tree.Forall2_eq in TRANSF; subst
               end).
 
+Ltac simplify :=
+  intros; subst;
+  repeat match goal with
+           | [H: OK _ = OK _ |- _] => inv H
+           | [H: bind _ _ = OK _ |- _] => monadInv H
+           | [H: _ /\ _ |- _] => destruct H
+         end;
+  subst; auto.
+
+Inductive optimize_rtl_program: forall (rtl: RTL.program) (ortl: RTL.program), Prop:=
+| rtlopt_tailcall: forall r1, optimize_rtl_program r1 (Tailcall.transf_program r1)
+| rtlopt_inlining: forall r1 r1' (TR_OK: Inlining.transf_program r1 = OK r1'),
+                     optimize_rtl_program r1 r1'
+| rtlopt_renumber: forall r1, optimize_rtl_program r1 (Renumber.transf_program r1)
+| rtlopt_constprop: forall r1, optimize_rtl_program r1 (Constprop.transf_program r1)
+| rtlopt_cse: forall r1 r1' (TR_OK: CSE.transf_program r1 = OK r1'),
+                optimize_rtl_program r1 r1'
+| rtlopt_deadcode: forall r1 r1' (TR_OK: Deadcode.transf_program r1 = OK r1'),
+                     optimize_rtl_program r1 r1'.
+
+Hint Constructors optimize_rtl_program.
+
 Definition rtl_opt_tree := Tree.change_one optimize_rtl_program.
 
 Lemma rtl_opt_tree_destruct:
@@ -83,15 +105,6 @@ Proof.
     (constructor; auto; eapply Tree.Forall2_implies;
     [ intros; right; apply H | apply Tree.Tree_Forall2_eq_same]).
 Qed.
-
-Ltac simplify :=
-  intros; subst;
-  repeat match goal with
-           | [H: OK _ = OK _ |- _] => inv H
-           | [H: bind _ _ = OK _ |- _] => monadInv H
-           | [H: _ /\ _ |- _] => destruct H
-         end;
-  subst; auto.
 
 Lemma rtl_opt_tree_reduce_simulation:
   forall tr tr' rtlprog
@@ -135,19 +148,6 @@ Proof.
     + des; subst; [eapply Deadcode_sig|]; eauto.
 Qed.
 
-Inductive match_state_refl (s:semantics): forall (st1 st2:state s), Prop :=
-| match_state_refl_intro: forall st, match_state_refl s st st.
-
-Lemma forward_simulation_refl:
-  forall sem, forward_simulation sem sem.
-Proof.
-  intros.
-  eapply forward_simulation_step; eauto; intros.
-  - eexists. split; eauto. apply (match_state_refl_intro _ s1).
-  - inv H; auto.
-  - eexists. inv H0. split; eauto. constructor.
-Qed.
-
 Lemma optimize_rtl_program_reduce_simulation:
   forall (rtlprog: RTL.program)
          (tr1 tr2: Tree.t RTL.program)
@@ -160,28 +160,120 @@ Proof.
   intros. generalize dependent rtlprog.
   induction ROPT; intros.
   - exploit rtl_opt_tree_reduce_simulation; eauto.
-  - exists rtlprog. exists (forward_simulation_refl (RTL.semantics rtlprog)); eauto.
+  - exists rtlprog. exists (forward_simulation_identity (RTL.semantics rtlprog)); eauto.
   - exploit IHROPT1; eauto. intros. des.
     exploit IHROPT2; eauto. intros. des.
     exists rtlprog'0.
     exists (compose_forward_simulation Hrtlsim' Hrtlsim'0); eauto.
 Qed.
 
-Lemma linker_correct_determinate_forward
+Lemma rtl_exists_frtl:
+  forall l rtlprog n asmprog
+         (TRANS: transf_rtl_program_opt n l rtlprog = OK asmprog),
+  exists frtlprog,
+    (rtc optimize_rtl_program) rtlprog frtlprog
+    /\ transf_rtl_program_to_asm_opt (OK frtlprog) = OK asmprog.
+Proof.
+  intros l. induction l; intros.
+  - unfold transf_rtl_program_opt in TRANS.
+    unfold transf_rtl_program_opt' in TRANS.
+    esplits; eauto.
+  - unfold transf_rtl_program_opt in TRANS.
+    unfold transf_rtl_program_opt' in TRANS; fold transf_rtl_program_opt' in TRANS.
+    destruct a; destruct r;
+    unfold print in TRANS;
+    simpl in TRANS;
+    unfold total_if, partial_if, time in TRANS;
+    destruct (b tt); try (by apply IHl in TRANS; eauto);
+    (match goal with [H: transf_rtl_program_opt' _ _ (?tr ?p) = _ |- _] =>
+                     destruct (tr p) eqn:TRRES;
+                     [|rewrite transf_rtl_program_opt'_error in H; inv H] end;
+     apply IHl in TRANS; des; inv TRRES;
+     match goal with [H: rtc optimize_rtl_program ?mp ?tp |- _] =>
+                     assert (TRANS': optimize_rtl_program rtlprog mp); try (by eauto) end;
+     esplits; [econs 3; [econs 1; apply TRANS'| apply TRANS] | eauto]).
+Qed.
+
+Lemma optimized_singleton_tree: forall p1 p2,
+            rtc optimize_rtl_program p1 p2 ->
+            rtc rtl_opt_tree (Tree.Tree_singleton p1) (Tree.Tree_singleton p2).
+Proof. i. induction H; [econs; econs|econs 2|econs 3]; eauto. Qed.
+
+Lemma rtl_tree_exists_frtl_tree:
+  forall rtltree asmtree rtlprog
+         (LINK: Tree.reduce (link_program Language_RTL) rtltree = Some rtlprog)
+         (T: Tree.Forall2 (fun a b => exists n, transf_rtl_program_opt n (fst b) a = OK (snd b)) rtltree asmtree),
+  exists frtltree,
+    rtc rtl_opt_tree rtltree frtltree
+    /\ Tree.Forall2 (fun a b => transf_rtl_program_to_asm_opt (OK a) = OK (snd b)) frtltree asmtree.
+Proof.
+  intros rtltree.
+  induction rtltree; intros.
+  - inv T. des.
+    eapply rtl_exists_frtl in Hpred. des.
+    exists (Tree.Tree_singleton frtlprog).
+    split; [| econs; eauto].
+    apply optimized_singleton_tree; eauto.
+  - apply Tree.reduce_composite in LINK. des. inv T.
+    eapply IHrtltree1 in FRED; eauto. des.
+    eapply IHrtltree2 in SRED; eauto. des.
+    esplits; [|econs; eauto].
+    econs 3.
+    + eapply Tree.rtc_change_one_attach_left; eauto.
+    + eapply Tree.rtc_change_one_attach_right; eauto.
+Qed.
+
+Lemma rtl_exists_forward_simulation:
+  forall p asmtree n
+         (rtlprog : RTL.program)
+         (Hrtlprog : Tree.reduce (link_program Language_RTL) p = Some rtlprog)
+         (T : Tree.Forall2
+                (fun (a : RTL.program) (b : opt_list * Asm.program) =>
+                   transf_rtl_program_opt n (fst b) a = OK (snd b)) p asmtree),
+  exists rtltree rtlprog'
+         (_: forward_simulation (RTL.semantics rtlprog) (RTL.semantics rtlprog')),
+    Tree.reduce (link_program Language_RTL) rtltree = Some rtlprog'
+    /\ Tree.Forall2 (fun a b => transf_rtl_program_to_asm_opt (OK a) = OK (snd b)) rtltree asmtree.
+Proof.
+  intros.
+  exploit rtl_tree_exists_frtl_tree; eauto.
+  { eapply Tree.Forall2_implies; eauto.
+    i. exists n. eauto. }
+  i; des.
+  exploit optimize_rtl_program_reduce_simulation; eauto. i; des.
+  esplits; eauto.
+Qed.
+
+Lemma asmtree_drop_flag:
+  forall mtree fasmtree
+         (T: Tree.Forall2 (fun (a : Mach.program) (b : opt_list * Asm.program) =>
+                             Asmgen.transf_program a = OK (snd b)) mtree fasmtree),
+  exists (asmtree: Tree.t Asm.program),
+    Tree.Forall2 (fun a b => Asmgen.transf_program a = OK b) mtree asmtree
+    /\ Tree.map snd fasmtree = asmtree.
+Proof.
+  intros.
+  exists (Tree.map snd fasmtree).
+  split; eauto.
+  generalize dependent mtree.
+  induction fasmtree; intros.
+  - inv T. econs. eauto.
+  - inv T. apply IHfasmtree1 in H0. apply IHfasmtree2 in H3.
+    unfold Tree.map; fold Tree.map.
+    econs; eauto.
+Qed.
+
+Lemma linker_correct_determinate_forward_optd
         ctree asmtree cprog
         (CLINK: Tree.reduce (link_program Language.Language_C) ctree = Some cprog)
-        (TRANSF: Tree.Forall2 compile_c_program ctree asmtree):
+        (TRANSF: Tree.Forall2 (fun s t => transf_c_program_opt (fst t) s = OK (snd t)) ctree asmtree):
   exists (asmprog:Asm.program)
     (_:forward_simulation (Cstrategy.semantics cprog) (Asm.semantics asmprog)),
-    Tree.reduce (link_program Language.Language_Asm) asmtree = Some asmprog.
+    Tree.reduce (link_program Language.Language_Asm) (Tree.map snd asmtree) = Some asmprog.
 Proof.
-  repeat intro.
-
   (* C *)
-  unfold compile_c_program in TRANSF.
-  eapply Tree.Tree_Forall2_split2 in TRANSF. des.
+  unfold transf_c_program_opt in TRANSF. clarify.
 
-  unfold transf_c_program_to_rtl in TRANSF. clarify.
   eapply Tree.Forall2_implies in T; [|apply SimplExprproof.SimplExpr_sepcomp_rel].
   eapply Tree.Forall2_reduce in T; eauto;
     [|eapply (@link_program_sepcomp_rel Language.Language_C Language.Language_Clight id)]; simplify;
@@ -190,7 +282,7 @@ Proof.
   apply SimplExprproof.transl_program_correct in Hclightsim.
 
   (* Clight *)
-  unfold transf_clight_program_to_rtl in TRANSF. clarify.
+  unfold transf_clight_program_opt in TRANSF. clarify.
 
   eapply Tree.Forall2_reduce in T1; eauto;
     [|eapply (transform_partial_program2_link_program Language.Language_Clight Language.Language_Clight)];
@@ -212,35 +304,33 @@ Proof.
   apply Cminorgenproof.transl_program_correct in Hcminorsim.
 
   (* Cminor *)
-  unfold transf_cminor_program_to_rtl in TRANSF. clarify.
+  unfold transf_cminor_program_opt in TRANSF. clarify.
 
   exploit Tree.Forall2_implies. apply Selectionproof.Selection_check_helpers. eauto.
   intro T_CH. apply Tree.Forall2_Forall in T_CH.
     
   eapply Tree.Forall_reduce in T_CH; [| apply Selectionproof.link_program_check_helpers|eauto].
-  eapply Tree.Forall2_implies in T; [|apply Selectionproof.Selection_sepcomp_rel].
+  eapply Tree.Forall2_implies in T0; [|apply Selectionproof.Selection_sepcomp_rel].
 
-  eapply Tree.Forall2_reduce in T; eauto;
+  eapply Tree.Forall2_reduce in T0; eauto;
     [|eapply (@link_program_sepcomp_rel Language.Language_Cminor Language.Language_CminorSel id)]; simplify;
     [|eapply Selection_sig; eauto].
 
-  destruct T as [cminorselprog [Hcminorselprog Hcminorselsim]].
+  destruct T0 as [cminorselprog [Hcminorselprog Hcminorselsim]].
 
   apply Selectionproof.transf_program_correct in Hcminorselsim;
     eauto using Selectionproof.check_helpers_correct.
 
-  eapply Tree.Forall2_reduce in TRANSF; eauto;
+  eapply Tree.Forall2_reduce in T; eauto;
     [|eapply (transform_partial_program2_link_program Language.Language_CminorSel Language.Language_RTL)];
     [|apply globfun_linkable_transf_partial_fundef];
     [|apply RTLgen_sig].
-  destruct TRANSF as [rtlprog0 [Hrtlprog0 Hrtlsim0]].
+  destruct T as [rtlprog0 [Hrtlprog0 Hrtlsim0]].
   apply RTLgenproof.transf_program_correct in Hrtlsim0.
 
 (* RTL *)
-  exploit optimize_rtl_program_reduce_simulation.
-  eauto. apply Tree.Tree_Forall2_rtc_rel_rtc_change_one. eauto.
-  intros. des.
-  unfold transf_rtl_program_to_asm in TRANSF1. clarify.
+  exploit rtl_exists_forward_simulation; eauto. intros [prtl1 [rtlprog1 [Hrtlprogsim1 [Hrtlprog1 TRANSF1]]]].
+  unfold transf_rtl_program_to_asm_opt in TRANSF1. clarify.
 
   eapply Tree.Forall2_reduce in T5; eauto;
     [|eapply (transform_partial_program2_link_program Language.Language_RTL Language.Language_LTL)];
@@ -274,6 +364,8 @@ Proof.
   eapply Stackingproof.transf_program_correct in Hmachsim; eauto;
     [|eexact Asmgenproof.return_address_exists; eassumption].
 
+  apply asmtree_drop_flag in TRANSF1. destruct TRANSF1 as [asmtree0 [TRANSF1 TEQ]].
+
   eapply Tree.Forall2_reduce in TRANSF1; eauto;
     [|eapply (transform_partial_program2_link_program Language.Language_Mach Language.Language_Asm)];
     [|apply globfun_linkable_transf_partial_fundef];
@@ -282,19 +374,20 @@ Proof.
   eapply Asmgenproof.transf_program_correct in Hasmsim; eauto.
 
   (* epilogue *)
-  exists asmprog. eexists; auto.
+  exists asmprog. eexists.
   repeat (auto; try (eapply compose_forward_simulation; [|eauto; fail])).
+  rewrite TEQ. eauto.
 Qed.
 
-Lemma linker_correct_determinate
+Lemma linker_correct_determinate_optd
         ctree asmtree cprog
         (CLINK: Tree.reduce (link_program Language.Language_C) ctree = Some cprog)
-        (TRANSF: Tree.Forall2 compile_c_program ctree asmtree):
+        (TRANSF: Tree.Forall2 (fun s t => transf_c_program_opt (fst t) s = OK (snd t)) ctree asmtree):
   exists (asmprog:Asm.program)
     (_:backward_simulation (atomic (Cstrategy.semantics cprog)) (Asm.semantics asmprog)),
-    Tree.reduce (link_program Language.Language_Asm) asmtree = Some asmprog.
+    Tree.reduce (link_program Language.Language_Asm) (Tree.map snd asmtree) = Some asmprog.
 Proof.
-  exploit linker_correct_determinate_forward; eauto.
+  exploit linker_correct_determinate_forward_optd; eauto.
   intros [asmprog [Hsim Hasmprog]]. exists asmprog.
   eexists; auto.
   apply forward_to_backward_simulation.
@@ -303,15 +396,15 @@ Proof.
   apply Asm.semantics_determinate.
 Qed.
 
-Theorem linker_correct
+Theorem linker_correct_optd
         ctree asmtree cprog
         (CLINK: Tree.reduce (link_program Language.Language_C) ctree = Some cprog)
-        (TRANSF: Tree.Forall2 compile_c_program ctree asmtree):
+        (TRANSF: Tree.Forall2 (fun s t => transf_c_program_opt (fst t) s = OK (snd t)) ctree asmtree):
   exists (asmprog:Asm.program)
     (_:backward_simulation (Csem.semantics cprog) (Asm.semantics asmprog)),
-    Tree.reduce (link_program Language.Language_Asm) asmtree = Some asmprog.
+    Tree.reduce (link_program Language.Language_Asm) (Tree.map snd asmtree) = Some asmprog.
 Proof.
-  exploit linker_correct_determinate; eauto.
+  exploit linker_correct_determinate_optd; eauto.
   intros [asmprog [Hsim Hasmprog]]. exists asmprog.
   eexists; eauto.
   apply compose_backward_simulation with (atomic (Cstrategy.semantics cprog)).
